import CompDiffPriv & HammingDistance -> BitVec

KA-CDP.ec
@@ -10,17 +10,99 @@ require import StdBigop. import Bigreal BRA.
 require import StdOrder. import RealOrder.
 require import StdRing. import RField.
 require BitWord FelTactic.
-require import HammingDistance.
+require import BitVec.
 require CompDiffPriv KeyAgreement.
 
 op input_len : {int | 0 < input_len} as gt0_input_len.
 
-clone BitWord as Input with
-    op n <- input_len
-proof gt0_n by apply gt0_input_len.
-
-
 
 (* CDP for hamming distance *)
 
+(* Alice's internal randomness *)
+
+op CDP_randA_len : {int | 0 < CDP_randA_len} as gt0_CDP_randA_len.
+
+clone BitWord as CDPRandA with 
+    op n <- CDP_randA_len
+proof gt0_n by apply gt0_CDP_randA_len.
+
+type randA_CDP = CDPRandA.word.
+
+op drandA_CDP : randA_CDP distr = CDPRandA.DWord.dunifin.
+
+lemma drandA_CDP_fu : is_full drandA_CDP.
+proof. apply CDPRandA.DWord.dunifin_fu. qed.
+
+lemma drandA_CDP_uni : is_uniform drandA_CDP.
+proof. apply CDPRandA.DWord.dunifin_uni. qed.
+
+lemma drandA_CDP_ll : is_lossless drandA_CDP.
+proof. apply CDPRandA.DWord.dunifin_ll. qed.
+
+
+(* Bob's internal randomness *)
+
+op CDP_randB_len : {int | 0 < CDP_randB_len} as gt0_CDP_randB_len.
+
+clone BitWord as CDPRandB with 
+    op n <- CDP_randB_len
+proof gt0_n by apply gt0_CDP_randB_len.
+
+type randB_CDP = CDPRandB.word.
+
+op drandB_CDP : randB_CDP distr = CDPRandB.DWord.dunifin.
+
+lemma drandB_CDP_fu : is_full drandB_CDP.
+proof. apply CDPRandB.DWord.dunifin_fu. qed.
+
+lemma drandB_CDP_uni : is_uniform drandB_CDP.
+proof. apply CDPRandB.DWord.dunifin_uni. qed.
+
+lemma drandB_CDP_ll : is_lossless drandB_CDP.
+proof. apply CDPRandB.DWord.dunifin_ll. qed.
+
+
+(* transcript *)
+
+op CDP_transc_len : {int | 0 < CDP_transc_len} as gt0_CDP_transc_len.
+
+clone BitWord as CDPTransc with 
+    op n <- CDP_transc_len
+proof gt0_n by apply gt0_CDP_transc_len.
+
+type transcript = CDPTransc.word.
+
+
+(* functionality of CDP *)
+
+op T_CDP : vec -> randA_CDP -> vec -> randB_CDP -> transcript.
+
+op outA_CDP : vec -> randA_CDP -> transcript -> int.
+
+op outB_CDP : vec -> randB_CDP -> transcript -> int.
+
 clone import CompDiffPriv as CDP with
+    type input <- vec,
+    op dinput <- dvec,
+    type output <- int,
+    type randA <- randA_CDP,
+    op drandA <- drandA_CDP,
+    type randB <- randB_CDP,
+    op drandB <- drandB_CDP,
+    type transcript <- transcript,
+    op F <- hd,
+    op adj <- adj,
+    op T <- T_CDP,
+    op outA <- outA_CDP,
+    op outB <- outB_CDP
+proof *.
+realize dinput_fu. apply dvec_full. qed.
+realize dinput_uni. apply dvec_uni. qed.
+realize dinput_ll. apply dvec_ll. qed.
+realize drandA_fu. apply drandA_CDP_fu. qed.
+realize drandA_uni. apply drandA_CDP_uni. qed.
+realize drandA_ll. apply drandA_CDP_ll. qed.
+realize drandB_fu. apply drandB_CDP_fu. qed.
+realize drandB_uni. apply drandB_CDP_uni. qed.
+realize drandB_ll. apply drandB_CDP_ll. qed.
+
